\section{Gabor Elementary function}
\begin{equation}
\psi(t) = \underbrace{e^{-\alpha ^2(t-t_0)^2}}_v\overbrace{e^{j2\pi f_0 t+\phi}}^w
\end{equation}

$v$ represents the probability function and $w$ represents simple harmonic oscillator.
$\Psi(f)$ is the GEF in the frequency domain. The GEF in the frequency domain is attained by taking the Fourier transform of the GEF.
\begin{equation*}
\Psi(f) = {\int_{-\infty}^{\infty}{\psi(t) e^{-j2\pi ft}dt}};
\Psi(f) = {\int_{-\infty}^{\infty}{e^{-\alpha ^2(t-t_0)^2}e^{j2\pi f_0 t+\phi} e^{-j2\pi ft}dt}}\\
\end{equation*}

\begin{equation*}
\Psi(f) = {\int_{-\infty}^{\infty}{e^{-\alpha ^2(t-t_0)^2}e^{j2\pi t(f_0-f) +\phi}dt}}
\end{equation*}

\begin{equation*}
\Psi(f) = e^\phi{\int_{-\infty}^{\infty}{e^{-\alpha ^2(t-t_0)^2}e^{j2\pi t(f_0-f) }dt}}
\end{equation*}

when $t_0$ is 0, then

\begin{equation}
\Psi(f) = e^\phi{\int_{-\infty}^{\infty}{e^{-\alpha ^2 t^2}e^{j2\pi t(f_0-f) }dt}}
\end{equation}


This is of the form.
\begin{equation*}
\int_{-\infty}^{\infty}e^{2bx - ax^2 }dx = \sqrt{\frac{\pi}{a}} e^\frac{b^2}{a}
\end{equation*}
where $b = j \pi(f_0-f)$ and $a = \alpha ^ 2$

\begin{equation*}
\Psi(f) = \sqrt{\frac{\pi}{\alpha ^2}} e^\frac{{(j\pi (f_0-f))}^2}{\alpha ^2}e^\phi
\end{equation*}
\begin{equation*}
\Psi(f) = \sqrt{\frac{\pi}{\alpha ^2}} e^{-{(\frac{\pi} {\alpha}})^2 ({f_0-f})^2+\phi}
\end{equation*}
$\alpha$ is connecting the GEF between time and frequency domain. $\psi(t)$ and $\Psi(f)$ occupies the minimum uncertainty in time and frequency domain.


\subsection{Proof: GEF has minimum uncertainty in the time-frequency domain}

I believe, we will better understand physical or mathematical concept by performing a step wise derivation. Let me do a step wise derivation to prove that GEF has a minimum uncertainty for a special case. Let me simplify the GEF by taking GEF at zero frequency, $t_0 = 0$ and $\phi = 0$,the Gabor elementary function and Fourier transform of GEF are given by
\begin{equation*}
\psi(t) = e^{-\alpha ^2 t^2}
\end{equation*}

\begin{equation*}
\Psi(f) = \sqrt{\frac{\pi}{\alpha ^2}} e^{-{(\frac{\pi} {\alpha}})^2 f^2}
\end{equation*}

Effective duration $\Delta t$ is given by:

\begin{equation*}
\Delta t = \sqrt{\frac{\int_{-\infty}^{\infty}{e^{-\alpha ^2 t^2} t^2  e^{-\alpha ^2 t^2} dt}}{\int_{-\infty}^{\infty}{e^{-\alpha ^2 t^2} e^{-\alpha ^2 t^2}dt}}} ;
\end{equation*}

Let me take the denominator first

\begin{equation*}
\int_{-\infty}^{\infty}{e^{-\alpha ^2 t^2} e^{-\alpha ^2 t^2}dt} =\int_{-\infty}^{\infty}{e^{-2\alpha ^2 t^2} dt}
\end{equation*}

The above equation is of the form and it only applies when $a > 0$

\begin{equation*}
\int_{-\infty}^{\infty}e^{-ax^2 }dx = \sqrt{\frac{\pi}{a}}
\end{equation*}

where $a = 2\alpha ^ 2$

\begin{equation*}
\int_{-\infty}^{\infty}{e^{-2\alpha ^2 t^2} dt} = \sqrt{\frac{\pi}{2\alpha ^ 2}}
\end{equation*}

Let me take the numerator now,

\begin{equation*}
\int_{-\infty}^{\infty}{e^{-\alpha ^2 t^2} t^2 e^{-\alpha ^2 t^2}dt} =\int_{-\infty}^{\infty}{t^2 e^{-2\alpha ^2 t^2} dt}
\end{equation*}

The above equation is of the form.
\begin{equation*}
\int_{-\infty}^{\infty}x^2 e^{- ax^2 }dx = \frac{1}{2}\sqrt{\frac{\pi}{a^3}}
\end{equation*}
where $a = 2\alpha ^ 2$
\begin{equation*}
\int_{-\infty}^{\infty}{t^2 e^{-2\alpha ^2 t^2} dt} = \frac{1}{2} \sqrt{\frac{\pi}{({2\alpha ^2})^3}} = \frac{\sqrt{\pi}}{4 \sqrt{2}\alpha ^3}
\end{equation*}

Let me apply both numerator and denominator value to get the effective duration $\Delta t$

\begin{equation*}
\Delta t = \sqrt{\frac{\frac{\sqrt{\pi}}{4 \sqrt{2}\alpha ^3}}{\sqrt{\frac{\pi}{2\alpha ^ 2}}}} ;
\end{equation*}

Straight forward steps to simply the value of $\Delta t$

\begin{equation*}
\Delta t =  \sqrt{\frac{\sqrt{\pi}}{4 \sqrt{2}\alpha ^3}{\sqrt{\frac{2\alpha ^ 2}{\pi}}}} ;
\end{equation*}

\begin{equation*}
\Delta t =  \sqrt{\frac{\sqrt{\pi}}{4 \sqrt{2}\alpha ^3}{\sqrt{\frac{2\alpha ^ 2}{\pi}}}} ;
\end{equation*}

\begin{equation*}
\Delta t =  \sqrt{\frac{1}{4 \alpha ^2}};
\end{equation*}


\begin{equation}
\Delta t =  \frac{1}{2 \alpha }
\end{equation}

Let me do the similar steps to calculate the effective frequency $\Delta f$. The frequency representation of the GEF is given by,

\begin{equation*}
\Psi(f) = \sqrt{\frac{\pi}{\alpha ^2}} e^{-{(\frac{\pi} {\alpha}})^2 f^2}
\end{equation*}

Effective frequency $\Delta f$ is given by,

\begin{equation*}
\Delta f = \sqrt{\frac{\int_{-\infty}^{\infty}{\sqrt{\frac{\pi}{\alpha ^2}} e^{-{(\frac{\pi} {\alpha}})^2 f^2} f^2 \sqrt{\frac{\pi}{\alpha ^2}} e^{-{(\frac{\pi} {\alpha}})^2 f^2} df}}{\int_{-\infty}^{\infty}{\sqrt{\frac{\pi}{\alpha ^2}} e^{-{(\frac{\pi} {\alpha}})^2 f^2}  \sqrt{\frac{\pi}{\alpha ^2}} e^{-{(\frac{\pi} {\alpha}})^2 f^2} df}}} ;
\end{equation*}

Let me take the denominator first.


\begin{equation*}
\int_{-\infty}^{\infty}{\sqrt{\frac{\pi}{\alpha ^2}} e^{-{(\frac{\pi} {\alpha}})^2 f^2}  \sqrt{\frac{\pi}{\alpha ^2}} e^{-{(\frac{\pi} {\alpha}})^2 f^2} df} = \frac{\pi}{\alpha ^2} \int_{-\infty}^{\infty}{ e^{-2{(\frac{\pi} {\alpha}})^2 f^2}df}
\end{equation*}



The above equation is of the form and it only applies when $a > 0$

\begin{equation*}
\int_{-\infty}^{\infty}e^{-ax^2 }dx = \sqrt{\frac{\pi}{a}}
\end{equation*}

where $a = 2(\frac{\pi}{\alpha})^ 2$

\begin{equation*}
\frac{\pi}{\alpha ^2} \int_{-\infty}^{\infty}{ e^{-2{(\frac{\pi} {\alpha}})^2 f^2}df} = \frac{\pi}{\alpha ^2} \sqrt{\frac{\pi}{2(\frac{\pi}{\alpha})^ 2}}
\end{equation*}

Let $\beta = \frac{\pi}{\alpha}$
\begin{equation*}
\frac{\pi}{\alpha ^2} \int_{-\infty}^{\infty}{ e^{-2{(\frac{\pi} {\alpha}})^2 f^2}df} = \frac{\beta}{\alpha} \sqrt{\frac{\pi}{2 \beta^ 2}} = \frac{1}{\alpha} \sqrt{\frac{\pi}{2 }}
\end{equation*}
Let me take the numerator now.
\begin{equation*}
\int_{-\infty}^{\infty}{\sqrt{\frac{\pi}{\alpha ^2}} e^{-{(\frac{\pi} {\alpha}})^2 f^2} f^2  \sqrt{\frac{\pi}{\alpha ^2}} e^{-{(\frac{\pi} {\alpha}})^2 f^2} df}
\end{equation*}

\begin{equation*}
=\frac{\pi}{\alpha ^2}\int_{-\infty}^{\infty}{ f^2 e^{-2{(\frac{\pi} {\alpha}})^2 f^2}  df}
\end{equation*}

Substitute $\beta$ in above equation.

\begin{equation*}
=\frac{\beta}{\alpha }\int_{-\infty}^{\infty}{ f^2 e^{-2 \beta ^2 f^2}  df}
\end{equation*}


The above equation is of the form.
\begin{equation*}
\int_{-\infty}^{\infty}x^2 e^{- ax^2 }dx = \frac{1}{2}\sqrt{\frac{\pi}{a^3}}
\end{equation*}
where $a = 2\beta ^ 2$
\begin{equation*}
 = \frac{\beta}{\alpha}\frac{1}{2}\sqrt\frac{\pi}{8\beta ^6 }
\end{equation*}

\begin{equation*}
 = \frac{\beta}{\alpha }\frac{\sqrt{\pi}}{4 \sqrt{2}\beta ^3}
\end{equation*}

Substitute the value of $\beta$

\begin{equation*}
 = \frac{1}{\alpha }\frac{\sqrt{\pi}}{4 \sqrt{2}\beta ^2}  = \frac{1}{\alpha }\frac{\sqrt{\pi} \alpha^2}{4 \sqrt{2}\pi ^2} = \frac{\sqrt{\pi} \alpha}{4 \sqrt{2}\pi ^2}
\end{equation*}

Apply the value of numerator and denominator of $\Delta f$

\begin{equation*}
\Delta f = \sqrt{\frac{\frac{\sqrt{\pi} \alpha}{4 \sqrt{2}\pi ^2}}{\frac{1}{\alpha} \sqrt{\frac{\pi}{2 }}}} = \sqrt{\frac{\sqrt{\pi} \alpha^2}{4 \sqrt{2}\pi ^2} \sqrt{\frac{2}{\pi }}}
\end{equation*}

Step wise simplification steps to get the value of $\Delta f$

\begin{equation*}
\Delta f =  \sqrt{\frac{\alpha ^2}{4 \pi ^2}}
\end{equation*}


\begin{equation}
\Delta f =  \frac{\alpha}{2 \pi}
\end{equation}

Apply both the value of $\Delta f$ and $\Delta t$ from equation (8) and equation (9)

\begin{equation*}
\Delta t \Delta f =  \frac{\alpha}{2 \pi} \frac{1}{2 \alpha }
\end{equation*}

\begin{equation*}
\boxed{\Delta t \Delta f =  \frac{1}{4 \pi}}
\end{equation*}

Hence the proof.
